# âš¡
# $a^2+(3a)^2$
## Notes
None.
## General Explanation
The derivation for this trick is similar to $a^2+(2a)^2$, except the final result is even more elegant. Expanding the expression, we get $a^2+(3a)^2=a^2+9a^2=10a^2$. Thus, we simply square a and multiply it by 10 to get $a^2+(3a)^2$.
## Example 1
$$8^2+24^2=$$
1. Since $a=8$, square it to get $a^2=64$
2. Multiply this result by 10 to get 640 ($64\times 10=640$)
3. Final Answer: **640**
## Example 2
$$13^2+26^2=$$
1. Since $a=13$, square it to get $a^2=169$
2. Multiply this result by 10 to get 1690 ($169\times 10=1690$)
3. Final Answer: **1690**

## Video Explanation(s)
None.

<br>*Written by: Steven Livingston*<br>
*Edited/Proofread by: n/a*